minuska/theories/try_match.v
@@ -1,0 +1,32 @@
+From Minuska Require Import
+    prelude
+    tactics
+    spec_syntax
+    spec_semantics
+    syntax_properties
+    basic_matching
+.
+
+
+Definition builtin_value_try_match_BuiltinOrVar
+    {Σ : Signature}
+    :
+    builtin_value -> BuiltinOrVar -> option Valuation :=
+fun b bv =>
+match bv with
+| bov_builtin b' => if (decide (b = b')) then Some ∅ else None
+| bov_variable x => Some (<[x := (aoo_operand _ _ b)]>∅)
+end.
+
+
+Definition pure_GroundTerm_try_match_BuiltinOrVar
+    {Σ : Signature}
+    :
+    AppliedOperator' symbol builtin_value -> BuiltinOrVar -> option Valuation
+:= fun t bov =>
+match bov with
+| bov_builtin b => None
+| bov_variable x =>
+    Some (<[x := (aoo_app _ _ t)]>∅)
+end.
+
